code/datatypes/maps.v
@@ -1,0 +1,34 @@
+Require Import  Datatypes EqNat Lists.List.
+Local Open Scope nat_scope.
+
+Notation " [ ] " := nil (format "[ ]").
+Notation " [ x ] " := (cons x nil).
+Notation "x :: l" := (cons x l) (at level 60, right associativity).
+Notation " [ x ; y ; .. ; z ] " := (cons x (cons y .. (cons z nil) ..)).
+
+Inductive id : Type :=
+  | Id : nat -> id.
+  
+Definition total_map (A:Type) := id -> A.
+
+Definition partial_map (A:Type) := total_map (option A).
+
+Definition tmap_empty {A:Type} (v : A) : total_map A :=
+  (fun _ => v).
+  
+
+Definition beq_id id1 id2 :=
+  match id1,id2 with
+    | Id n1, Id n2 => beq_nat n1 n2
+  end.
+  
+Definition t_update {A:Type} (m : total_map A)
+                    (x : id) (v : A) :=
+  fun x' => if beq_id x x' then v else m x'.
+
+Definition emptymap {A:Type} : partial_map A :=
+  tmap_empty None.
+
+Definition update {A:Type} (m : partial_map A)
+                  (x : id) (v : A) :=
+  t_update m x (Some v).
